theories/theories/utp_rel.thy
@@ -6,7 +6,7 @@
 header {* Relational Predicates *}
 
 theory utp_rel
-imports "../generic/utp_gen_pred" "../generic/utp_eval_tactic"
+imports "../generic/utp_generic"
 begin
 
 context GEN_PRED
@@ -22,35 +22,17 @@ definition WF_CONDITION :: "('VALUE, 'TYPE) ALPHA_PREDICATE set" where
 "WF_CONDITION =
  {p . p \<in> WF_RELATION \<and> p = (\<exists>p DASHED . p)}"
 
-subsection {* Substitution *}
-
-text {* The definitions below should probably be in the predicate locale. *}
-
-definition SubstB ::
-  "('TYPE VAR \<Rightarrow> 'TYPE VAR) \<Rightarrow>
-   ('VALUE, 'TYPE) BINDING \<Rightarrow>
-   ('VALUE, 'TYPE) BINDING" where
-"\<lbrakk>ss \<in> VAR_SUBST;
- b \<in> WF_BINDING\<rbrakk> \<Longrightarrow>
- SubstB ss b = b \<circ> (inv ss)"
-
-definition SubstP ::
-  " ('VALUE, 'TYPE) ALPHA_PREDICATE \<Rightarrow>
-   ('TYPE VAR \<Rightarrow> 'TYPE VAR) \<Rightarrow>
-   ('VALUE, 'TYPE) ALPHA_PREDICATE" ("_[_]" [200]) where
-"\<lbrakk>ss \<in> VAR_SUBST;
- p \<in> WF_ALPHA_PREDICATE\<rbrakk> \<Longrightarrow>
- SubstP p ss = (ss ` (\<alpha> p), (SubstB ss) ` (\<beta> p))"
+subsection {* Substitutions *}
 
 definition SS1 :: "'TYPE VAR \<Rightarrow> 'TYPE VAR" where
 "SS1 v = (
- if dashes (name v) = 1 then (VAR.dash v) else
- if dashes (name v) = 2 then (VAR.undash v) else v)"
+ if dashes (name v) = 1 then (dash v) else
+ if dashes (name v) = 2 then (undash v) else v)"
 
 definition SS2 :: "'TYPE VAR \<Rightarrow> 'TYPE VAR" where
 "SS2 v = (
- if dashes (name v) = 0 then VAR.dash (VAR.dash v) else
- if dashes (name v) = 2 then VAR.undash (VAR.undash v) else v)"
+ if dashes (name v) = 0 then dash (dash v) else
+ if dashes (name v) = 2 then undash (undash v) else v)"
 
 subsection {* Relational Operators *}
 
@@ -72,167 +54,46 @@ definition SemiR ::
    ('VALUE, 'TYPE) ALPHA_PREDICATE" (infixr ";" 140) where
 "r1 \<in> WF_RELATION \<and>
  r2 \<in> WF_RELATION \<and>
- COMPOSABLE (\<alpha> r1) (\<alpha> r1) \<longrightarrow>
+ COMPOSABLE (\<alpha> r1) (\<alpha> r2) \<longrightarrow>
  r1 ; r2 = (\<exists>-p dash ` (out (\<alpha> r1)) . r1[SS1] \<and>p r2[SS2])"
+
+text {* Configure theorems for the predicate proof tactic. *}
+
+declare CondR_def [eval]
+declare SemiR_def [eval]
 
 subsection {* Theorems *}
 
-text {* Variable Substitution *}
+subsubsection {* Restrictions *}
 
-theorem VAR_SUBST_inv_closure [simp] :
-"ss \<in> VAR_SUBST \<Longrightarrow> (inv ss) \<in> VAR_SUBST"
+theorem WF_RELATION_WF_ALPHA_PREDICATE :
+"p \<in> WF_RELATION \<Longrightarrow> p \<in> WF_ALPHA_PREDICATE"
+apply (simp add: WF_RELATION_def)
+done
+
+declare WF_RELATION_WF_ALPHA_PREDICATE [eval]
+
+subsubsection {* Substitutions *}
+
+theorem SS1_VAR_SUBST [simp] :
+"SS1 \<in> VAR_SUBST"
+apply (simp add: SS1_def_raw)
 apply (simp add: VAR_SUBST_def)
-apply (safe)
-apply (auto intro: bij_imp_bij_inv)
-apply (drule_tac x = "inv ss v" in spec)
-apply (erule subst)
-apply (simp add: surj_f_inv_f bij_def)
-done
+apply (simp_all add: dash_def undash_def)
+apply (rule bijI)
+apply (rule injI)
+sorry
 
-theorem VAR_SUBST_inv_inv [simp] :
-"ss \<in> VAR_SUBST \<Longrightarrow> inv (inv ss) = ss"
+theorem SS2_VAR_SUBST [simp] :
+"SS2 \<in> VAR_SUBST"
+apply (simp add: SS2_def_raw)
 apply (simp add: VAR_SUBST_def)
-apply (simp add: inv_inv_eq)
-done
+apply (simp_all add: dash_def undash_def)
+apply (rule bijI)
+apply (rule injI)
+sorry
 
-theorem VAR_SUBST_ss_inv [simp] :
-"ss \<in> VAR_SUBST \<Longrightarrow> ss (inv ss x) = x"
-apply (simp add: VAR_SUBST_def)
-apply (simp add: surj_f_inv_f bij_def)
-done
-
-theorem VAR_SUBST_inv_ss [simp] :
-"ss \<in> VAR_SUBST \<Longrightarrow> inv ss (ss x) = x"
-apply (simp add: VAR_SUBST_def)
-apply (simp add: inv_f_f bij_def)
-done
-
-theorem VAR_SUBST_image_inv [simp] :
-"ss \<in> VAR_SUBST \<Longrightarrow> ss ` (inv ss) ` a = a"
-apply (simp add: image_def)
-apply (auto)
-done
-
-theorem VAR_SUBST_inv_image [simp] :
-"ss \<in> VAR_SUBST \<Longrightarrow> (inv ss) ` ss ` a = a"
-apply (simp add: image_def)
-apply (auto)
-done
-
-text {* Binding Substitution *}
-
-theorem SubstB_closure [simp] :
-"\<lbrakk>ss \<in> VAR_SUBST;
- b \<in> WF_BINDING\<rbrakk> \<Longrightarrow>
- SubstB ss b \<in> WF_BINDING"
-apply (simp add: SubstB_def WF_BINDING_def)
-apply (simp add: VAR_SUBST_def)
-apply (safe)
-apply (drule_tac x = "inv ss v" in spec)
-apply (subgoal_tac "type (inv ss v) = type v")
-apply (simp)
-apply (drule_tac x = "inv ss v" in spec)
-apply (erule subst)
-apply (simp add: surj_f_inv_f bij_def)
-done
-
-theorem SubstB_cancel1 [simp] :
-"\<lbrakk>ss \<in> VAR_SUBST;
- b \<in> WF_BINDING\<rbrakk> \<Longrightarrow>
- SubstB (inv ss) (SubstB ss b) = b"
-apply (subgoal_tac "SubstB ss b \<in> WF_BINDING")
-apply (simp add: SubstB_def)
-apply (rule ext)
-apply (simp_all)
-done
-
-theorem SubstB_cancel2 [simp] :
-"\<lbrakk>ss \<in> VAR_SUBST;
- b \<in> WF_BINDING\<rbrakk> \<Longrightarrow>
- SubstB ss (SubstB (inv ss) b) = b"
-apply (subgoal_tac "SubstB (inv ss) b \<in> WF_BINDING")
-apply (simp add: SubstB_def)
-apply (rule ext)
-apply (simp_all)
-done
-
-text {* Predicate Substitution *}
-
-theorem SubstP_closure_lemma :
-"\<lbrakk>ss \<in> VAR_SUBST;
- b1 \<in> WF_BINDING;
- b2 \<in> WF_BINDING\<rbrakk> \<Longrightarrow>
- SubstB ss b1 \<cong> b2 on ss ` a \<longrightarrow> b1 \<cong> SubstB (inv ss) b2 on a"
-apply (simp add: beta_equiv_def)
-apply (simp add: SubstB_def)
-done
-
-theorem SubstP_closure [simp] :
-"\<lbrakk>p \<in> WF_ALPHA_PREDICATE;
- ss \<in> VAR_SUBST\<rbrakk> \<Longrightarrow>
- p[ss] \<in> WF_ALPHA_PREDICATE"
-apply (simp add: SubstP_def)
-apply (simp add: WF_ALPHA_PREDICATE_def)
-apply (safe)
--- {* Subgoal 1 *}
-apply (auto simp: WF_ALPHABET_def)
--- {* Subgoal 2 *}
-apply (simp add: WF_BINDING_SET_def)
-apply (safe)
--- {* Subgoal 2.1 *}
-apply (subgoal_tac "xa \<in> WF_BINDING")
-apply (simp)
-apply (auto) [1]
--- {* Subgoal 2.2 *}
-apply (simp (no_asm_simp) add: image_def)
-apply (rule_tac x = "SubstB (inv ss) b2" in bexI)
-apply (simp)
-apply (drule_tac x = "b1" in bspec)
-apply (assumption)
-apply (drule_tac x = "SubstB (inv ss) b2" in bspec)
-apply (simp)
-apply (subgoal_tac "b1 \<cong> SubstB (inv ss) b2 on \<alpha> p")
-apply (simp)
-apply (subst SubstP_closure_lemma)
-apply (auto)
-done
-
-theorem SubstP_alphabet [simp] :
-"\<lbrakk>p \<in> WF_ALPHA_PREDICATE;
- ss \<in> VAR_SUBST\<rbrakk> \<Longrightarrow>
- \<alpha> p[ss] = ss ` (\<alpha> p)"
-apply (simp add: SubstP_def)
-done
-
-theorem EvalP_SubstP [eval] :
-"\<lbrakk>p \<in> WF_ALPHA_PREDICATE;
- ss \<in> VAR_SUBST;
- b \<in> WF_BINDING\<rbrakk> \<Longrightarrow>
- EvalP p[ss] b = EvalP p (SubstB (inv ss) b)"
-apply (simp add: EvalP_def)
-apply (simp add: SubstP_def)
-apply (simp add: image_def)
-apply (safe)
-apply (subgoal_tac "x \<in> WF_BINDING")
-apply (simp)
-apply (simp add: WF_BINDING_predicate)
-apply (rule_tac x = "SubstB (inv ss) b" in bexI)
-apply (simp)
-apply (assumption)
-done
-
-text {* Conditional *}
-
-theorem CondR_closure [simp] :
-"\<lbrakk>p1 \<in> WF_RELATION;
- p2 \<in> WF_RELATION;
- b \<in> WF_CONDITION;
- \<alpha> p1 = \<alpha> p2;
- \<alpha> b \<subseteq> \<alpha> p1\<rbrakk> \<Longrightarrow>
- (p1 \<triangleleft> b \<triangleright> p2) \<in> WF_RELATION"
-apply (simp add: CondR_def)
-apply (simp add: WF_RELATION_def WF_CONDITION_def)
-done
+subsubsection {* Alphabet Theorems *}
 
 theorem CondR_alphabet [simp]:
 "\<lbrakk>p1 \<in> WF_RELATION;
@@ -246,33 +107,95 @@ apply (simp add: WF_RELATION_def WF_CONDITION_def)
 apply (auto)
 done
 
-declare CondR_def [eval]
+theorem SemiR_alphabet [simp] :
+"r1 \<in> WF_RELATION \<and>
+ r2 \<in> WF_RELATION \<and>
+ COMPOSABLE (\<alpha> r1) (\<alpha> r2) \<longrightarrow>
+ \<alpha> (r1 ; r2) = in (\<alpha> r1) \<union> out (\<alpha> r2)"
+apply (simp add: SemiR_def)
+apply (simp add: WF_RELATION_def)
+apply (simp add: WF_ALPHABET_alphabet)
+apply (safe)
+-- {* Subgoal 1 *}
+apply (case_tac "xa \<in> DASHED")
+apply (simp add: SS1_def DASHED_def)
+apply (simp add: out_alphabet_def DASHED_def)
+apply (subgoal_tac "xa \<in> UNDASHED")
+apply (simp add: SS1_def in_alphabet_def UNDASHED_def)
+apply (auto)
+-- {* Subgoal 2 *}
+sorry
+
+(***********************)
+(* REVIEWED UNTIL HERE *)
+(***********************)
+
+subsubsection {* Closure Theorems *}
+
+theorem CondR_closure [simp] :
+"\<lbrakk>p1 \<in> WF_RELATION;
+ p2 \<in> WF_RELATION;
+ b \<in> WF_CONDITION;
+ \<alpha> p1 = \<alpha> p2;
+ \<alpha> b \<subseteq> \<alpha> p1\<rbrakk> \<Longrightarrow>
+ (p1 \<triangleleft> b \<triangleright> p2) \<in> WF_RELATION"
+apply (simp add: CondR_def)
+apply (simp add: WF_RELATION_def WF_CONDITION_def)
+done
+
+theorem SemiR_closure [simp] :
+"r1 \<in> WF_RELATION \<and>
+ r2 \<in> WF_RELATION \<and>
+ COMPOSABLE (\<alpha> r1) (\<alpha> r2) \<longrightarrow>
+ r1 ; r2 \<in> WF_RELATION"
+apply (simp add: SemiR_def)
+apply (simp add: WF_RELATION_def)
+apply (simp add: WF_ALPHABET_alphabet)
+apply (auto)
+-- {* Subgoal 1 *}
+apply (case_tac "xa \<in> DASHED")
+apply (simp add: SS1_def DASHED_def)
+apply (simp add: out_alphabet_def DASHED_def)
+apply (subgoal_tac "xa \<in> UNDASHED")
+apply (simp add: SS1_def UNDASHED_def)
+apply (auto)
+-- {* Subgoal 2 *}
+apply (case_tac "xa \<in> UNDASHED")
+apply (simp add: WF_ALPHABET_alphabet COMPOSABLE_def)
+apply (simp add: SS2_def UNDASHED_def)
+apply (simp add: in_alphabet_def UNDASHED_def)
+apply (subgoal_tac "xa \<in> DASHED")
+apply (simp add: SS2_def DASHED_def)
+apply (auto)
+done
+
+theorem WF_RELATION_TrueP [simp] :
+"\<lbrakk>a \<in> WF_ALPHABET;
+ a \<subseteq> UNDASHED \<union> DASHED\<rbrakk> \<Longrightarrow>
+ true a \<in> WF_RELATION"
+apply (simp only: WF_RELATION_def)
+apply (auto)
+done
+
+theorem WF_RELATION_FalseP [simp] :
+"\<lbrakk>a \<in> WF_ALPHABET;
+ a \<subseteq> UNDASHED \<union> DASHED\<rbrakk> \<Longrightarrow>
+ false a \<in> WF_RELATION"
+apply (simp only: WF_RELATION_def)
+apply (auto)
+done
 
 subsection {* Proof Experiments *}
 
-theorem SubstP_lemma1 [simp] :
-"\<lbrakk>p \<in> WF_ALPHA_PREDICATE;
- ss \<in> VAR_SUBST\<rbrakk> \<Longrightarrow>
- p[ss][inv ss] = p"
-apply (utp_pred_taut_tac)
-done
-
-theorem SubstP_lemma2 [simp] :
-"\<lbrakk>p1 \<in> WF_ALPHA_PREDICATE;
- p2 \<in> WF_ALPHA_PREDICATE;
- ss \<in> VAR_SUBST\<rbrakk> \<Longrightarrow>
- (p1 \<and>p p2)[ss] = p1[ss] \<and>p p2[ss]"
+theorem
+"\<lbrakk>r \<in> WF_RELATION;
+ a \<in> WF_ALPHABET;
+ a \<subseteq> UNDASHED \<union> DASHED;
+ COMPOSABLE a (\<alpha> r)\<rbrakk> \<Longrightarrow>
+ false a ; r = false ((in a) \<union> out (\<alpha> r))"
 apply (utp_pred_eq_tac)
 apply (auto)
-done
-
-theorem SubstP_lemma3 [simp] :
-"\<lbrakk>p \<in> WF_ALPHA_PREDICATE;
- ss \<in> VAR_SUBST\<rbrakk> \<Longrightarrow>
- taut [p] \<Leftrightarrow>p [p[ss]]"
-apply (utp_pred_taut_tac)
-apply (auto)
--- {* This proof is more tricky! *}
+-- {* TODO: See if the proof of the subgoals can be automated. *}
 oops
 end
 end
