theories/generic/utp_subst.thy
@@ -1,0 +1,296 @@
+(******************************************************************************)
+(* Title: utp/theories/utp_subst.thy                                          *)
+(* Author: Frank Zeyda, University of York                                    *)
+(******************************************************************************)
+
+header {* Substitution *}
+
+theory utp_subst
+imports utp_gen_pred utp_eval_tactic
+begin
+
+context GEN_PRED
+begin
+
+subsection {* Variable Substitutions *}
+
+text {* Substitutions are total bijections and have to respect typing. *}
+
+definition VAR_SUBST :: "('TYPE VAR \<Rightarrow> 'TYPE VAR) set" where
+"VAR_SUBST = {ss . bij ss \<and> (\<forall> v . type (ss v) = type v)}"
+
+subsection {* Binding Substitution *}
+
+definition SubstB ::
+  "('TYPE VAR \<Rightarrow> 'TYPE VAR) \<Rightarrow>
+   ('VALUE, 'TYPE) BINDING \<Rightarrow>
+   ('VALUE, 'TYPE) BINDING" where
+"\<lbrakk>ss \<in> VAR_SUBST; b \<in> WF_BINDING\<rbrakk> \<Longrightarrow>
+ SubstB ss b = b \<circ> (inv ss)"
+
+subsection {* Predicate Substitution *}
+
+definition SubstP ::
+  " ('VALUE, 'TYPE) ALPHA_PREDICATE \<Rightarrow>
+   ('TYPE VAR \<Rightarrow> 'TYPE VAR) \<Rightarrow>
+   ('VALUE, 'TYPE) ALPHA_PREDICATE" ("_[_]" [200]) where
+"\<lbrakk>ss \<in> VAR_SUBST; p \<in> WF_ALPHA_PREDICATE\<rbrakk> \<Longrightarrow>
+ SubstP p ss = (ss ` (\<alpha> p), (SubstB ss) ` (\<beta> p))"
+
+subsection {* Theorems *}
+
+text {* General Functions *}
+
+theorem bij_comp_inject :
+"bij g \<Longrightarrow> (f1 \<circ> g = f2 \<circ> g) = (f1 = f2)"
+apply (safe)
+apply (rule ext)
+apply (subgoal_tac "\<exists> y . x = g y")
+apply (clarify)
+apply (drule_tac x = "y" in fun_cong)
+apply (auto)
+apply (simp add: bij_def surj_def)
+done
+
+declare bij_imp_bij_inv [simp, intro!]
+
+subsubsection {* Variable Substitution *}
+
+theorem VAR_SUBST_inv [simp] :
+"ss \<in> VAR_SUBST \<Longrightarrow> (inv ss) \<in> VAR_SUBST"
+apply (simp add: VAR_SUBST_def)
+apply (safe)
+apply (drule_tac x = "inv ss v" in spec)
+apply (erule subst)
+apply (simp add: surj_f_inv_f bij_def)
+done
+
+theorem VAR_SUBST_inv_inv [simp] :
+"ss \<in> VAR_SUBST \<Longrightarrow> inv (inv ss) = ss"
+apply (simp add: VAR_SUBST_def)
+apply (simp add: inv_inv_eq)
+done
+
+theorem VAR_SUBST_ss_inv [simp] :
+"ss \<in> VAR_SUBST \<Longrightarrow> ss (inv ss x) = x"
+apply (simp add: VAR_SUBST_def)
+apply (simp add: surj_f_inv_f bij_def)
+done
+
+theorem VAR_SUBST_inv_ss [simp] :
+"ss \<in> VAR_SUBST \<Longrightarrow> inv ss (ss x) = x"
+apply (simp add: VAR_SUBST_def)
+apply (simp add: inv_f_f bij_def)
+done
+
+theorem VAR_SUBST_image_inv [simp] :
+"ss \<in> VAR_SUBST \<Longrightarrow> ss ` (inv ss) ` a = a"
+apply (simp add: image_def)
+apply (auto)
+done
+
+theorem VAR_SUBST_inv_image [simp] :
+"ss \<in> VAR_SUBST \<Longrightarrow> (inv ss) ` ss ` a = a"
+apply (simp add: image_def)
+apply (auto)
+done
+
+theorem VAR_SUBST_in_image_simp [simp] :
+"\<lbrakk>ss \<in> VAR_SUBST\<rbrakk> \<Longrightarrow> (ss x \<in> ss ` a) = (x \<in> a)"
+apply (simp add: VAR_SUBST_def)
+apply (auto simp: bij_def inj_eq)
+done
+
+theorem VAR_SUBST_WF_BINDING [simp] :
+"\<lbrakk>b \<in> WF_BINDING; ss \<in> VAR_SUBST\<rbrakk> \<Longrightarrow>
+ b \<circ> ss \<in> WF_BINDING"
+apply (simp add: VAR_SUBST_def WF_BINDING_def)
+apply (safe)
+apply (drule_tac x = "ss v" in spec)
+apply (drule_tac x = "v" in spec)
+apply (auto)
+done
+
+text {* Binding Substitution *}
+
+theorem SubstB_closure [simp] :
+"\<lbrakk>ss \<in> VAR_SUBST;
+ b \<in> WF_BINDING\<rbrakk> \<Longrightarrow>
+ SubstB ss b \<in> WF_BINDING"
+apply (simp add: SubstB_def)
+done
+
+theorem SubstsB_inject [simp]:
+"\<lbrakk>b1 \<in> WF_BINDING;
+ b2 \<in> WF_BINDING;
+ ss \<in> VAR_SUBST\<rbrakk> \<Longrightarrow>
+ (SubstB ss b1 = SubstB ss b2) = (b1 = b2)"
+apply (simp add: SubstB_def)
+apply (simp add: VAR_SUBST_def)
+apply (simp add: bij_comp_inject)
+done
+
+theorem SubstB_inv_cancel1 [simp] :
+"\<lbrakk>ss \<in> VAR_SUBST;
+ b \<in> WF_BINDING\<rbrakk> \<Longrightarrow>
+ SubstB (inv ss) (SubstB ss b) = b"
+apply (subgoal_tac "SubstB ss b \<in> WF_BINDING")
+apply (simp add: SubstB_def)
+apply (rule ext)
+apply (simp_all)
+done
+
+theorem SubstB_inv_cancel2 [simp] :
+"\<lbrakk>ss \<in> VAR_SUBST;
+ b \<in> WF_BINDING\<rbrakk> \<Longrightarrow>
+ SubstB ss (SubstB (inv ss) b) = b"
+apply (subgoal_tac "SubstB (inv ss) b \<in> WF_BINDING")
+apply (simp add: SubstB_def)
+apply (rule ext)
+apply (simp_all)
+done
+
+subsubsection {* Predicate Substitution *}
+
+theorem SubstP_alphabet [simp] :
+"\<lbrakk>p \<in> WF_ALPHA_PREDICATE;
+ ss \<in> VAR_SUBST\<rbrakk> \<Longrightarrow>
+ \<alpha> p[ss] = ss ` (\<alpha> p)"
+apply (simp add: SubstP_def)
+done
+
+text {* Could the following be useful in other places too? Examine! *}
+
+theorem SubstP_closure_lemma :
+"\<lbrakk>ss \<in> VAR_SUBST;
+ b1 \<in> WF_BINDING;
+ b2 \<in> WF_BINDING\<rbrakk> \<Longrightarrow>
+ SubstB ss b1 \<cong> b2 on ss ` a \<longrightarrow> b1 \<cong> SubstB (inv ss) b2 on a"
+apply (simp add: beta_equiv_def)
+apply (simp add: SubstB_def)
+done
+
+theorem SubstP_closure [simp] :
+"\<lbrakk>p \<in> WF_ALPHA_PREDICATE;
+ ss \<in> VAR_SUBST\<rbrakk> \<Longrightarrow>
+ p[ss] \<in> WF_ALPHA_PREDICATE"
+apply (simp add: SubstP_def)
+apply (simp add: WF_ALPHA_PREDICATE_def)
+apply (safe)
+-- {* Subgoal 1 *}
+apply (auto simp: WF_ALPHABET_def)
+-- {* Subgoal 2 *}
+apply (simp add: WF_BINDING_SET_def)
+apply (safe)
+-- {* Subgoal 2.1 *}
+apply (subgoal_tac "xa \<in> WF_BINDING")
+apply (simp)
+apply (auto) [1]
+-- {* Subgoal 2.2 *}
+apply (simp (no_asm_simp) add: image_def)
+apply (rule_tac x = "SubstB (inv ss) b2" in bexI)
+apply (simp)
+apply (drule_tac x = "b1" in bspec)
+apply (assumption)
+apply (drule_tac x = "SubstB (inv ss) b2" in bspec)
+apply (simp)
+apply (subgoal_tac "b1 \<cong> SubstB (inv ss) b2 on \<alpha> p")
+apply (simp)
+apply (subst SubstP_closure_lemma)
+apply (auto)
+done
+
+theorem EvalP_SubstP [eval] :
+"\<lbrakk>p \<in> WF_ALPHA_PREDICATE;
+ ss \<in> VAR_SUBST;
+ b \<in> WF_BINDING\<rbrakk> \<Longrightarrow>
+ EvalP p[ss] b = EvalP p (SubstB (inv ss) b)"
+apply (simp add: EvalP_def)
+apply (simp add: SubstP_def)
+apply (simp add: image_def)
+apply (safe)
+apply (subgoal_tac "x \<in> WF_BINDING")
+apply (simp)
+apply (simp add: WF_BINDING_predicate)
+apply (rule_tac x = "SubstB (inv ss) b" in bexI)
+apply (simp)
+apply (assumption)
+done
+
+theorem EvalP_SubstsP_SubstB [simp] :
+"\<lbrakk>p \<in> WF_ALPHA_PREDICATE;
+ b \<in> WF_BINDING;
+ ss \<in> VAR_SUBST\<rbrakk> \<Longrightarrow>
+ EvalP p[ss] (SubstB ss b) = EvalP p b"
+apply (simp add: EvalP_def)
+apply (simp add: SubstP_def)
+apply (simp add: image_def)
+apply (auto)
+apply (subgoal_tac "x \<in> WF_BINDING")
+apply (simp)
+apply (simp add: WF_BINDING_predicate)
+done
+
+subsubsection {* Algebraic Laws *}
+
+theorem SubstP_inverse :
+"\<lbrakk>p \<in> WF_ALPHA_PREDICATE;
+ ss \<in> VAR_SUBST\<rbrakk> \<Longrightarrow>
+ p[ss][inv ss] = p"
+apply (utp_pred_taut_tac)
+done
+
+theorem SubstP_AndP_distr :
+"\<lbrakk>p1 \<in> WF_ALPHA_PREDICATE;
+ p2 \<in> WF_ALPHA_PREDICATE;
+ ss \<in> VAR_SUBST\<rbrakk> \<Longrightarrow>
+ (p1 \<and>p p2)[ss] = p1[ss] \<and>p p2[ss]"
+apply (utp_pred_eq_tac)
+apply (auto)
+done
+
+theorem Closure_SubstP :
+"\<lbrakk>p \<in> WF_ALPHA_PREDICATE;
+ ss \<in> VAR_SUBST\<rbrakk> \<Longrightarrow>
+ [p[ss]] = ([p] :: ('VALUE, 'TYPE) ALPHA_PREDICATE)"
+apply (utp_pred_taut_tac)
+apply (auto)
+-- {* Can we automate discharging the following residual subgoal? *}
+apply (drule_tac x = "SubstB ss x" in bspec)
+apply (simp)
+apply (simp add: SubstB_def)
+apply (subgoal_tac
+  "EvalP p ((b \<oplus> x \<circ> (inv ss) on ss ` \<alpha> p) \<circ> ss) \<oplus> x on - \<alpha> p")
+apply (subgoal_tac
+  "x = ((b \<oplus> x \<circ> (inv ss) on ss ` \<alpha> p) \<circ> ss) \<oplus> x on - \<alpha> p")
+apply (simp)
+apply (rule ext)
+apply (simp add: comp_def)
+apply (case_tac "ss xa \<in> ss ` \<alpha> p")
+apply (simp)
+apply (simp)
+apply (simp_all add: EvalP_override)
+done
+
+subsection {* Proof Experiments *}
+
+text {*
+  The following proof illustrate how we use a mixture of algebraic laws and
+  the proof strategy for predicates to proof more complex properties. For now
+  the strategy alone is not powerful enough to prove the theorem by itself.
+*}
+
+theorem SubstP_lemma1 :
+"\<lbrakk>p1 \<in> WF_ALPHA_PREDICATE;
+ p2 \<in> WF_ALPHA_PREDICATE;
+ ss \<in> VAR_SUBST\<rbrakk> \<Longrightarrow>
+ taut [p1 \<Leftrightarrow>p p2] \<Leftrightarrow>p [p1[ss] \<Leftrightarrow>p p2[ss]]"
+apply (subgoal_tac "p1[ss] \<Leftrightarrow>p p2[ss] = (p1 \<Leftrightarrow>p p2)[ss]")
+apply (simp)
+apply (simp add: Closure_SubstP)
+apply (utp_pred_taut_tac)
+apply (utp_pred_eq_tac)
+apply (auto)
+done
+end
+end
